vera/VerilogSimpl.v
@@ -1,0 +1,301 @@
+From vera Require Import Verilog.
+From vera Require Import Decidable.
+From vera Require Import Tactics.
+From vera Require Import Bitvector.
+From vera Require Import Common.
+Import Verilog.
+(* From vera Require VerilogSemantics. *)
+
+From ExtLib Require Import Structures.Monads.
+
+From Stdlib Require Import BinNums.
+From Stdlib Require Import ZArith.
+From Stdlib Require Import String.
+From Stdlib Require Import List.
+
+From Equations Require Import Equations.
+
+Import MonadLetNotation.
+Import ListNotations.
+Local Open Scope monad_scope.
+Local Open Scope string.
+Local Open Scope list.
+
+Program Definition equalized_shiftop {w1 w2}
+    (wf : (w1 > 0)%N) op (lhs : expression w1) (rhs : expression w2)
+    : expression w1 :=
+  Resize w1
+    (ShiftOp op
+      (Resize (N.max w1 w2) lhs _)
+      (Resize (N.max w1 w2) rhs _)
+      _ _)
+    _.
+Next Obligation. lia. Qed.
+Next Obligation. lia. Qed.
+Next Obligation. lia. Qed.
+Next Obligation. lia. Qed.
+
+Equations simpl_expr {w} : expression w -> expression w := {
+  | UnaryOp op e => UnaryOp op (simpl_expr e)
+  | ArithmeticOp op lhs rhs => ArithmeticOp op (simpl_expr lhs) (simpl_expr rhs)
+  | BitwiseOp op lhs rhs => BitwiseOp op (simpl_expr lhs) (simpl_expr rhs)
+  | @ShiftOp w1 w2 op lhs rhs _ _ with dec (w1 = w2) => {
+    | left E => ShiftOp op (simpl_expr lhs) (simpl_expr rhs) _ _
+    | right _ =>
+      (* Shift operand widths must match in SMTLIB *)
+      equalized_shiftop _ op (simpl_expr lhs) (simpl_expr rhs)
+  }
+  | Concatenation e1 e2 => Concatenation (simpl_expr e1) (simpl_expr e2)
+  | Replication n e =>
+    (* TODO: Convert replications to concats *)
+    Replication n (simpl_expr e)
+  | Conditional cond ifT ifF => Conditional (simpl_expr cond) (simpl_expr ifT) (simpl_expr ifF)
+  | RangeSelect vec hi lo _ wf => RangeSelect (simpl_expr vec) hi lo _ wf
+  | BitSelect_width vec idx _ _ =>
+    (* No variable bitselect in SMTLIB. Also, the shift we add must be balanced, as above. *)
+    BitSelect_const
+      (equalized_shiftop _ BinaryShiftRight (simpl_expr vec) idx)
+      0 ltac:(lia)
+  | BitSelect_const vec idx _ => BitSelect_const (simpl_expr vec) idx _
+  | Resize to expr _ => Resize to (simpl_expr expr) _
+  | IntegerLiteral w val => IntegerLiteral w val
+  | NamedExpression var => NamedExpression var
+}.
+Next Obligation. lia. Qed.
+
+Definition simpl_vmodule (v : vmodule) : vmodule :=
+  {|
+    Verilog.modName := Verilog.modName v;
+    Verilog.modVariableDecls := Verilog.modVariableDecls v;
+    Verilog.modBody := map
+      (fun '(AlwaysComb (BlockingAssign lhs rhs)) => AlwaysComb (BlockingAssign lhs (simpl_expr rhs)))
+      (Verilog.modBody v)
+  |}.
+
+From vera Require Import VerilogSemantics.
+Import (notations) RegisterState.
+From vera Require Import Tactics.
+
+From Stdlib Require Import Logic.ProofIrrelevance.
+From Stdlib Require Import Sorting.Permutation.
+
+Import CombinationalOnly.
+Import EqNotations.
+Local Open Scope verilog.
+
+Lemma convert_extend_to_N from to (xbv : XBV.xbv from) val :
+  (to >= from)%N ->
+  XBV.to_N xbv = Some val ->
+  XBV.to_N (convert to xbv) = Some val.
+Proof.
+  intros.
+  funelim (convert to xbv); [idtac|lia|idtac].
+  - destruct_rew. simpl. apply XBV.extend_to_N. assumption.
+  - destruct_rew. simpl. assumption.
+Qed.
+
+Lemma convert_extend_to_N_none from to (xbv : XBV.xbv from) :
+  (to >= from)%N ->
+  XBV.to_N xbv = None ->
+  XBV.to_N (convert to xbv) = None.
+Proof.
+  intros.
+  funelim (convert to xbv).
+  - destruct_rew. simpl. apply XBV.extend_to_N_none2. assumption.
+  - lia.
+  - destruct_rew. simpl. assumption.
+Qed.
+
+Lemma convert_shr_convert n1 n2 (xbv : XBV.xbv n1) shamt :
+  (n2 >= n1)%N ->
+  convert n1 (XBV.shr (convert n2 xbv) shamt) = XBV.shr xbv shamt.
+Proof.
+  intros.
+  funelim (convert n2 xbv); [idtac|lia|idtac].
+  all: destruct_rew; simpl.
+  - funelim (convert from (XBV.shr (XBV.concat (XBV.zeros (to - from)) value) shamt)); [lia|idtac|lia].
+    apply XBV.extr_shr_extend.
+  - funelim (convert from (XBV.shr value shamt)); [lia|lia|idtac].
+    rewrite <- eq_rect_eq. reflexivity.
+Qed.
+
+Lemma convert_shl_convert n1 n2 (xbv : XBV.xbv n1) shamt :
+  (n2 >= n1)%N ->
+  convert n1 (XBV.shl (convert n2 xbv) shamt) = XBV.shl xbv shamt.
+Proof.
+  intros.
+  funelim (convert n2 xbv); [idtac|lia|idtac].
+  all: destruct_rew; simpl.
+  - funelim (convert from (XBV.shl (XBV.concat (XBV.zeros (to - from)) value) shamt)); [lia|idtac|lia].
+    apply XBV.extr_shl_extend.
+  - funelim (convert from (XBV.shl value shamt)); [lia|lia|idtac].
+    rewrite <- eq_rect_eq. reflexivity.
+Qed.
+
+Lemma convert_exes n1 n2 :
+  (n2 <= n1)%N ->
+  convert n2 (XBV.exes n1) = XBV.exes n2.
+Proof.
+  intros.
+  funelim (convert n2 (XBV.exes n1)).
+  - lia.
+  - apply XBV.extr_exes.
+  - destruct_rew. reflexivity.
+Qed.
+
+Lemma eval_equalized_shiftop {w1 w2} regs op wf (lhs : expression w1) (rhs : expression w2) :
+  eval_expr regs (equalized_shiftop wf op lhs rhs)
+    = eval_shiftop op (eval_expr regs lhs) (eval_expr regs rhs).
+Proof.
+  unfold equalized_shiftop.
+  simp eval_expr. simpl.
+  generalize (eval_expr regs lhs). clear lhs. intro lhs.
+  generalize (eval_expr regs rhs). clear rhs. intro rhs.
+  funelim (eval_shiftop op lhs rhs).
+  all: simp eval_shiftop.
+  all: match type of Heq with
+       | (_ = Some _) => apply convert_extend_to_N with (to := N.max n1 n2) in Heq
+       | (_ = None) => apply convert_extend_to_N_none with (to := N.max n1 n2) in Heq
+       end; [|lia].
+  all: rewrite Heq; simpl.
+  - apply convert_shr_convert. lia.
+  - apply convert_exes. lia.
+  - apply convert_shl_convert. lia.
+  - apply convert_exes. lia.
+  - apply convert_shl_convert. lia.
+  - apply convert_exes. lia.
+Qed.
+
+(* TODO: Move me to bitvectors *)
+Lemma bitOf_exes i n : XBV.bitOf i (XBV.exes n) = RawXBV.X.
+Proof. apply nth_repeat. Qed.
+
+Hint Rewrite bitOf_exes : xbv.
+
+(* TODO: Move me to bitvectors *)
+Lemma shr_empty n : RawXBV.shr [] n = [].
+Proof. destruct n. all: simp shr. all: reflexivity. Qed.
+
+Hint Rewrite shr_empty : shr.
+
+(* TODO: Move me to bitvectors *)
+Lemma bitOf_shr w n (xbv : XBV.xbv w) :
+  (n < w)%N ->
+  XBV.bitOf 0 (XBV.shr xbv n) =
+  XBV.bitOf (N.to_nat n) xbv.
+Proof.
+  intros Hin_bounds.
+  unfold XBV.shr, XBV.bitOf.
+  XBV.bitvector_erase. subst.
+  N_to_nat.
+  unfold RawXBV.bitOf.
+  funelim (RawXBV.shr bv n); expect 3.
+  1, 2: reflexivity.
+  simpl in *.
+  rewrite <- H by lia.
+  apply app_nth1.
+  pose proof (RawXBV.shr_size n bs).
+  crush.
+Qed.
+
+Hint Rewrite bitOf_shr using lia : xbv.
+
+Lemma simpl_expr_correct {w} regs (e : expression w) :
+  eval_expr regs (simpl_expr e) = eval_expr regs e.
+Proof.
+  funelim (simpl_expr e).
+  all: simp eval_expr in *; simpl in *.
+  all: repeat match goal with
+       | [ Hinduct : forall r, eval_expr r (simpl_expr _) = eval_expr r _ |- _ ] =>
+         rewrite Hinduct in *
+       end.
+  all: try reflexivity.
+  all: clear Heqcall.
+  - (* Variable bitselect *)
+    rewrite eval_equalized_shiftop.
+    simp eval_shiftop.
+    unfold select_bit.
+    destruct (XBV.to_N (eval_expr regs idx)) eqn:E; simpl.
+    + (* well-defined *)
+      rewrite bitOf_shr by (apply XBV.to_N_max_bound in E; lia).
+      rewrite H.
+      reflexivity.
+    + (* X index *)
+      rewrite bitOf_exes.
+      XBV.bitvector_erase.
+      reflexivity.
+  - (* shifts *)
+    rewrite eval_equalized_shiftop.
+    rewrite H. rewrite H0.
+    reflexivity.
+Qed.
+
+Lemma equalized_shiftop_reads_reads_permutation w1 w2 wf op (lhs : expression w1) (rhs : expression w2) :
+  Permutation (expr_reads (equalized_shiftop wf op lhs rhs)) (expr_reads lhs ++ expr_reads rhs).
+Proof. unfold equalized_shiftop. simp expr_reads. reflexivity. Qed.
+
+Lemma simpl_expr_reads_permutation w (e : expression w) :
+  Permutation (expr_reads (simpl_expr e)) (expr_reads e).
+Proof.
+  funelim (simpl_expr e); clear Heqcall.
+  all: simp expr_reads.
+  all: try rewrite equalized_shiftop_reads_reads_permutation.
+  all: repeat match goal with
+       | [ H : Permutation (expr_reads (simpl_expr _)) (expr_reads _) |- _ ] =>
+         rewrite H
+       end.
+  all: reflexivity.
+Qed.
+
+Lemma simpl_vmodule_same_inputs v :
+  module_inputs (simpl_vmodule v) = module_inputs v.
+Proof. apply Verilog.module_inputs_same. reflexivity. Qed.
+
+Lemma simpl_vmodule_same_outputs v :
+  module_outputs (simpl_vmodule v) = module_outputs v.
+Proof. apply Verilog.module_outputs_same. reflexivity. Qed.
+
+Lemma simpl_vmodule_same_variables v :
+  modVariables (simpl_vmodule v) = modVariables v.
+Proof. apply Verilog.module_variables_same. reflexivity. Qed.
+
+Lemma simpl_vmodule_correct init v :
+  run_vmodule (simpl_vmodule v) init = run_vmodule v init.
+Proof.
+  unfold run_vmodule, mk_initial_state.
+  simpl.
+  rewrite simpl_vmodule_same_inputs.
+
+  rewrite sort_module_items_map; expect 3; cycle 1.
+  {
+    intros [[lhs rhs]].
+    simp module_item_reads module_item_writes statement_reads statement_writes expr_reads.
+    apply simpl_expr_reads_permutation.
+  }
+  {
+    intros [[lhs rhs]].
+    simp module_item_reads module_item_writes statement_reads statement_writes expr_reads.
+    reflexivity.
+  }
+
+  destruct (sort_module_items (module_inputs v) (modBody v));
+    simpl; [|reflexivity].
+  generalize (init // module_inputs v). clear init v.
+  induction l; intros r; [reflexivity|].
+  destruct a; expect 1. destruct s; expect 1.
+  simpl. simp exec_module_body exec_module_item exec_statement. simpl.
+  simp exec_module_body.
+  rewrite simpl_expr_correct.
+  apply IHl.
+Qed.
+
+Import ExactEquivalence.
+
+Theorem simpl_vmodule_exact_equivalence v :
+  simpl_vmodule v ~~~ v.
+Proof.
+  apply exact_by_output_equality.
+  - reflexivity.
+  - intros initial. rewrite simpl_vmodule_correct.
+    reflexivity.
+Qed.
